Common/CResult.v
@@ -1,0 +1,142 @@
+Require Import CBase.
+From stdpp Require Import option.
+
+(** The point of this module is to keep the [sum] type symmetric and use this to
+    assign a meaning to success and error (and a corresponding monad instance)
+
+    The naming is intended to match Ocaml's result as Haskell uses Either which
+    is similar to the regular [sum].
+ *)
+
+Section Result.
+
+  (** The error type is first so that [result E] is a monad *)
+  Context {E A : Type}.
+
+  Inductive result : Type :=
+  | Ok (val : A)
+  | Error (err : E).
+
+  Definition get_Ok (r : result) : option A :=
+    match r with
+    | Ok val => Some val
+    | Error err => None
+    end.
+
+  Definition get_Error (r : result) : option E :=
+    match r with
+    | Ok val => None
+    | Error err => Some err
+    end.
+
+  (** Takes an option but convert [None] into the provided error *)
+  Definition res_from_opt (e : E) : option A -> result :=
+  from_option Ok (Error e).
+
+  (* For convenience *)
+  Definition res_to_opt := get_Ok.
+
+  Definition res_from_suml (s : A + E) : result :=
+    match s with
+    | inl val => Ok val
+    | inr err => Error err
+    end.
+
+  Definition res_from_sumr (s : E + A) : result :=
+    match s with
+    | inr val => Ok val
+    | inl err => Error err
+    end.
+
+  Definition res_to_suml (r : result) : A + E :=
+    match r with
+    | Ok val => inl val
+    | Error err => inr err
+    end.
+
+  Definition res_to_sumr (r : result) : E + A :=
+    match r with
+    | Ok val => inr val
+    | Error err => inl err
+    end.
+
+  Lemma res_from_to_suml (s : A + E) : res_to_suml (res_from_suml s) = s.
+  Proof using. by destruct s. Qed.
+
+  Lemma res_to_from_suml (r : result) : res_from_suml (res_to_suml r) = r.
+  Proof using. by destruct r. Qed.
+
+  Lemma res_from_to_sumr (s : E + A) : res_to_sumr (res_from_sumr s) = s.
+  Proof using. by destruct s. Qed.
+
+  Lemma res_to_from_sumr (r : result) : res_from_sumr (res_to_sumr r) = r.
+  Proof using. by destruct r. Qed.
+
+
+  (** [is_Err] and [is_Ret] are doing the same as [is_Some] but for results *)
+  Definition is_Error (r : result) := ∃ err, r = Error err.
+  #[export] Instance is_Error_Decision (r : result) : Decision (is_Error r).
+  Proof.
+    refine (match r with | Error _ => left _ | _ => right _ end);
+      unfold is_Error;
+      naive_solver.
+  Defined.
+
+  Definition is_Ok (r : result) := ∃ val, r = Ok val.
+  #[export] Instance is_Ok_Decision (r : result) : Decision (is_Ok r).
+  Proof.
+    refine (match r with | Ok _ => left _ | _ => right _ end);
+      unfold is_Ok;
+      naive_solver.
+  Defined.
+
+  (** Unpack a result into any monad that supports that error type *)
+  Definition unpack_result `{MThrow E M, MRet M} (r : result) : M A :=
+    match r with
+    | Ok val => mret val
+    | Error err => mthrow err
+    end.
+
+End Result.
+Arguments result : clear implicits.
+
+
+(** * Result as monad *)
+Section ResultMonad.
+  Context {E : Type}.
+
+  Global Instance result_ret : MRet (result E) := @Ok E.
+
+  Global Instance result_throw : MThrow E (result E) := @Error E.
+
+  Global Instance result_bind : MBind (result E) :=
+    λ _ _ f r,
+      match r with
+      | Ok val => f val
+      | Error err => Error err
+      end.
+
+  Global Instance result_join : MJoin (result E) :=
+    λ _ r,
+      match r with
+      | Error err => Error err
+      | Ok (Error err) => Error err
+      | Ok (Ok a) => Ok a
+      end.
+
+  Global Instance result_fmap : FMap (result E) :=
+    λ _ _  f r,
+      match r with
+      | Ok val => Ok (f val)
+      | Error err => Error err
+      end.
+
+End ResultMonad.
+
+(** * Error map *)
+
+Definition mapE {E E' A} (f : E → E') (r : result E A) : result E' A :=
+  match r with
+  | Ok val => Ok val
+  | Error err => Error (f err)
+  end.
