Common/Effects.v
@@ -1,0 +1,441 @@
+(** This file provide support for handling algebraic effects.
+    It uses UIP *)
+
+Require Import CBase CBool.
+From stdpp Require Import base.
+From stdpp Require Import fin.
+From stdpp Require Import vector.
+
+(** UIP is need for this theory to be usable *)
+Require Export Eqdep.
+Require Export Program.Equality.
+
+From Equations Require Import Equations.
+
+
+
+
+
+(** An effected is a function from Type to Type that take the return type of the
+    effect and give the type of all calls that could return that return type.
+
+    This is voluntarily NOT universe polymorphic. It should probably be Set →
+    Set to be honest. *)
+Definition eff := Type → Type.
+
+(** Generic interface for calling an algebraic effect in a monad *)
+Class MCall (Eff : eff) (M : Type → Type) := mcall : ∀ {A}, Eff A → M A.
+#[global] Arguments mcall {_ _ _ _} _ : assert.
+#[global] Instance: Params (@mcall) 4 := {}.
+#[global] Hint Mode MCall - ! : typeclass_instances.
+
+(** Call a non returning effect. This is not necessarily a failure, so this
+    doesn't automatically implement MThrow *)
+Definition mcall_noret `{EmptyT T, MBind M, MCall Eff M} (call : Eff T) {A} :
+    M A :=
+  x ← mcall call;
+  match emptyT x with end.
+
+
+(** Generic sub-effect judgment, in theory this looks like MCall, but make both
+the same causes universes problems. In addition they need a different Hint Mode
+*)
+Class SubEff (Eff Eff' : eff) := eff_inj : ∀ {A}, Eff A → Eff' A.
+#[global] Arguments eff_inj {_ _ _ _} _ : assert.
+#[global] Instance: Params (@eff_inj) 4 := {}.
+#[global] Hint Mode SubEff ! ! : typeclass_instances.
+
+#[global] Instance SubEff_default Eff : SubEff Eff Eff | 100 := λ _ x, x.
+
+(* TODO, this might need to be a Hint Extern *)
+Definition MCall_SubEff {E} `{MCall E' M} `{SubEff E E'} : MCall E M :=
+  λ A e, mcall (eff_inj e : E' A).
+
+#[export] Hint Extern 5 (MCall ?E ?M) =>
+  tryif (is_evar E) then fail else class_apply MCall_SubEff
+  : typeclass_instances.
+
+
+
+
+(** Scope for effect notation *)
+Declare Scope effect_scope.
+Delimit Scope effect_scope with eff.
+Bind Scope effect_scope with eff.
+Open Scope effect_scope.
+
+Notation "x .T1" := (projT1 x) (at level 1, left associativity, format "x .T1").
+Notation "x .T2" := (projT2 x) (at level 1, left associativity, format "x .T2").
+
+(** For any effect value, either a value to be returned exists, or the effect is
+    an exception and can be converted to the associated exception type *)
+Module Eff.
+  Section Eff.
+    Context {Eff : eff}.
+
+    (** * Effect equality *)
+    Definition eq {T T'} (call : Eff T) (call' : Eff T') :=
+      existT T call = existT T' call'.
+    Infix "=ₑ" := eq (at level 70, no associativity) : effect_scope.
+
+    Definition conv_call {T T'} (eq : T = T') (call : Eff T) : Eff T' :=
+      eq_rect T Eff call T' eq.
+
+    Definition conv_ret {T T'} (eq : T = T') (ret : T) : T' :=
+      eq_rect T (λ x, x) ret T' eq.
+
+    Definition eq_type {T T'} {call : Eff T} {call' : Eff T'} :
+      call =ₑ call' → T = T' := @eq_sigT_fst _ _ _ _ _ _.
+
+    Definition eq_call {T} {call call': Eff T} :
+      call =ₑ call' → call = call' := inj_pair2 _ _ _ _ _.
+
+    Definition eq_call_rew {T} {call call': Eff T} :
+      call =ₑ call' ↔ call = call'.
+    Proof using. split; [apply eq_call | naive_solver]. Qed.
+
+    Lemma existT_eq_type {a b : sigT Eff} : a = b → a.T1 = b.T1.
+    Proof using. scongruence. Qed.
+
+    Lemma existT_eq_simplify (a : sigT Eff) (c : Eff a.T1) :
+      a = existT _ c → a.T2 = c.
+    Proof using.
+      intro H.
+      destruct a.
+      by dependent destruction H.
+    Qed.
+
+
+    (** * Effect Decision *)
+    Class Decision :=
+      decide_eq T T' (c : Eff T) (c' : Eff T') :: base.Decision (c =ₑ c').
+
+    #[global] Instance eff_decision_sigT `{Decision} : EqDecision (sigT Eff).
+    Proof using. intros [] []. solve_decision. Defined.
+
+    #[global] Instance eff_decision_eff `{Decision} T : EqDecision (Eff T).
+    Proof using.
+      refine (λ x y, dec_if (decide (x =ₑ y))).
+      - by apply eq_call.
+      - naive_solver.
+    Defined.
+
+
+    (** * Effect wellformedness
+
+          An effect is wellformed if we have DecisionT for all type that it
+          could ask as return type. In other words if for all effects we can
+          decide if has an empty return type or not *)
+    Class Wf := wf : ∀ T, Eff T → DecisionT T.
+
+
+    (** * Exception representation.
+
+        The goal of this typeclass is to represent all effects that cannot be
+        returned to as a single exception type
+     *)
+    Class Exc := {
+        exc : Type;
+        exc2eff : exc → sigT Eff;
+        eff2exc : ∀ {T}, Eff T → option exc;
+        exc_wf : ∀ e T call,
+          exc2eff e = existT T call ↔ eff2exc call = Some e;
+        exc_empty : ∀ T (call : Eff T), is_Some (eff2exc call) ↔ (T → False)
+        }.
+    Context {E : Exc}.
+
+
+    Lemma exc_empty_helper `{Inhabited T} P: ¬ P → P ↔ (T → False).
+    Proof using. sfirstorder. Qed.
+
+    Lemma exc_no_return T (call : Eff T) : is_Some (eff2exc call) → T → False.
+    Proof using. by rewrite exc_empty. Qed.
+
+    #[global] Instance exc2eff_inj : Inj (=) (=) (exc2eff).
+    Proof using.
+      intros x y H.
+      destruct (exc2eff x) eqn:Heqn.
+      hfcrush use:exc_wf.
+    Qed.
+
+    Definition exc2call (e : exc) := (exc2eff e).T2.
+
+    Lemma exc2call_wf {T} (c : Eff T) e:
+      eff2exc c = Some e ↔ c =ₑ exc2call e.
+    Proof using.
+      unfold exc2call.
+      unfold eq.
+      rewrite <- sigT_eta.
+      sfirstorder use:exc_wf.
+    Qed.
+
+    Lemma ret_or_exc_exc2call e : eff2exc (exc2call e) = Some e.
+    Proof using.
+      unfold exc2call.
+      rewrite <- exc_wf.
+      rewrite <- sigT_eta.
+      reflexivity.
+    Qed.
+
+    #[global] Instance eff2exc_type_empty e : EmptyT (Eff.exc2eff e).T1.
+    Proof using.
+      unfold EmptyT.
+      rewrite <- exc_empty.
+      eexists.
+      by apply ret_or_exc_exc2call.
+    Qed.
+
+    Lemma exc_type_empty e : (exc2eff e).T1 → False.
+    Proof using.
+      intro T.
+      destruct (exc2eff e) eqn:He.
+      eapply exc_no_return.
+      - rewrite exc_wf in He. naive_solver.
+      - assumption.
+    Qed.
+
+
+  End Eff.
+
+  Infix "=ₑ" := Eff.eq (at level 70, no associativity) : effect_scope.
+  #[global] Hint Mode Exc ! : typeclasses_instances.
+  #[global] Arguments Exc : clear implicits.
+  #[global] Arguments exc _ {_}.
+  #[global] Hint Mode Wf ! : typeclasses_instances.
+  #[global] Arguments Wf : clear implicits.
+  #[global] Hint Mode Decision ! : typeclass_instances.
+  #[global] Arguments Decision : clear implicits.
+  #[global] Arguments decide_eq {_ _ _ _} _ _ : simpl never, assert.
+
+  #[global] Hint Rewrite @ret_or_exc_exc2call : eff.
+
+  Ltac Wf_decisionT_apply T :=
+    match goal with
+    | call : ?Eff T |- _ =>
+        let H := fresh "H" in
+        enough (Wf Eff) as H; first apply (H T call)
+    end.
+  #[global] Hint Extern 5 (DecisionT ?T) =>
+           Wf_decisionT_apply T : typeclass_instances.
+
+  Tactic Notation "simplify_eff_eq" "in" ident(H) :=
+    match type of H with
+    | _ = @existT Type ?Eff ?T ?call =>
+        is_var T;
+        let H' := fresh "H" in
+        pose proof (existT_eq_type H) as H'; cbn in H';
+        subst T;
+        apply (@existT_eq_simplify Eff) in H
+    | @existT Type ?Eff ?T ?call = _ =>
+        is_var T;
+        let H' := fresh "H" in
+        pose proof (existT_eq_type H) as H'; cbn in H';
+        subst T;
+        symmetry in H;
+        apply (@existT_eq_simplify Eff) in H;
+        symmetry in H
+    | @Eff.eq _ ?T _ ?call _ =>
+        is_var T;
+        let H' := fresh "H" in
+        pose proof (Eff.eq_type H) as H';
+        subst T;
+        apply Eff.eq_call in H
+    | @Eff.eq _ _ ?T _ ?call =>
+        is_var T;
+        let H' := fresh "H" in
+        pose proof (Eff.eq_type H) as H';
+        subst T;
+        apply Eff.eq_call in H
+    end.
+
+  Tactic Notation "simplify_eff_eq" :=
+    match goal with
+    | H : Eff.eq _ _ |- _ => simplify_eff_eq in H
+    | H : _ = @existT Type _ _ _ |- _ => simplify_eff_eq in H
+    | H : @existT Type _ _ _ = _ |- _ => simplify_eff_eq in H
+    end.
+
+
+  Section Plus.
+    Context {Eff : eff}.
+    Context {Eff' : eff}.
+
+    Definition plus : eff := λ T, (Eff T + Eff' T)%type.
+
+    #[global] Instance plus_wf `{Wf Eff, Wf Eff'} : Wf plus.
+    Proof using. intros T x. destruct x; naive_solver. Qed.
+
+    #[global] Instance plus_dec `{Decision Eff, Decision Eff'} : Decision plus.
+    Proof using.
+      intros T T' c c'.
+      refine (match c, c' with
+              | inl a, inl b => dec_if (decide (a =ₑ b))
+              | inr a, inr b => dec_if (decide (a =ₑ b))
+              | _, _ => right _
+              end);
+        hauto lq:on simp+:simplify_eff_eq.
+    Defined.
+
+    #[global] Program Instance plus_exc `{Exc Eff, Exc Eff'} : Exc plus :=
+      { exc := exc Eff + exc Eff';
+        exc2eff e := match e return sigT plus with
+                     | inl x => existT _ (inl (exc2eff x).T2)
+                     | inr x => existT _ (inr (exc2eff x).T2)
+                     end;
+        eff2exc _ e := match e with
+                     | inl x => inl <$> eff2exc x
+                     | inr x => inr <$> eff2exc x
+                     end
+      }.
+    Next Obligation.
+      repeat case_split;
+        (split; intro Heq; [simplify_eff_eq | rewrite fmap_Some in Heq]);
+        sauto q:on dep:on use:exc_wf db:eff.
+    Qed.
+    Next Obligation.
+      case_split;
+        rewrite fmap_is_Some;
+        rewrite exc_empty;
+        reflexivity.
+    Qed.
+
+    (** Effect injection. Most of the time, the correct version is the left one,
+        so it has a higher priority *)
+    #[global] Instance subeff_plusl `{SubEff E Eff} : SubEff E plus | 10 :=
+      λ _ e, inl (eff_inj e).
+    #[global] Instance subeff_plusr `{SubEff E Eff'} : SubEff E plus | 20 :=
+      λ _ e, inr (eff_inj e).
+  End Plus.
+  #[global] Arguments plus : clear implicits.
+
+End Eff.
+Export (hints, notations, ltac.notations) Eff.
+#[export] Hint Rewrite @Eff.exc2call_wf : eff.
+#[export] Hint Rewrite @Eff.ret_or_exc_exc2call : eff.
+#[export] Hint Rewrite @Eff.eq_call_rew : eff.
+
+Infix "+ₑ" := Eff.plus (at level 50, left associativity) : effect_scope.
+Infix "=ₑ" := Eff.eq (at level 70, no associativity) : effect_scope.
+
+
+Infix "=ₑ" := Eff.eq (at level 70, no associativity) : effect_scope.
+Infix "=ₑ@{ A }" := (@Eff.eq A _)
+  (at level 70, only parsing, no associativity) : effect_scope.
+
+
+Notation "(=ₑ)" := Eff.eq (only parsing) : effect_scope.
+Notation "( X =ₑ.)" := (Eff.eq X) (only parsing) : effect_scope.
+Notation "(.=ₑ X )" := (λ Y, Y =ₑ X) (only parsing) : effect_scope.
+Notation "(≠ₑ)" := (λ X Y, ¬X =ₑ Y) (only parsing) : effect_scope.
+Notation "X ≠ₑ Y":= (¬X =ₑ Y) (at level 70, no associativity) : effect_scope.
+Notation "( X ≠ₑ.)" := (λ Y, X ≢ Y) (only parsing) : effect_scope.
+Notation "(.≠ₑ X )" := (λ Y, Y ≢ X) (only parsing) : effect_scope.
+
+Notation "(=ₑ@{ Eff } )" := (@Eff.eq Eff _ _) (only parsing) : effect_scope.
+Notation "(≠ₑ@{ Eff } )" := (λ X Y, ¬X =ₑ@{Eff} Y) (only parsing) : effect_scope.
+Notation "X ≠ₑ@{ Eff } Y":= (¬X =ₑ@{ Eff } Y)
+  (at level 70, only parsing, no associativity) : effect_scope.
+
+(** * Tactics about effects *)
+
+(** A version of [decide_eq] but for [Eff.eq]. Similarly, it expects the effect
+    type (Inductive) to be destroyed before the call *)
+Ltac decide_eff_eq :=
+  lazymatch goal with
+  | |- Decision (?f ?a ?b ?c ?d ?e ?f ?g =ₑ ?f ?a' ?b' ?c' ?d' ?e' ?f' ?g') =>
+      decide_field a a'; [ .. |
+      decide_field b b'; [ .. |
+      decide_field c c'; [ .. |
+      decide_field d d'; [ .. |
+      decide_field e e'; [ .. |
+      decide_field f f'; [ .. |
+      decide_field g g'; [ .. |
+      left; reflexivity]]]]]]]
+  | |- Decision (?f ?a ?b ?c ?d ?e ?f =ₑ ?f ?a' ?b' ?c' ?d' ?e' ?f') =>
+      decide_field a a'; [ .. |
+      decide_field b b'; [ .. |
+      decide_field c c'; [ .. |
+      decide_field d d'; [ .. |
+      decide_field e e'; [ .. |
+      decide_field f f'; [ .. |
+      left; reflexivity]]]]]]
+  | |- Decision (?f ?a ?b ?c ?d ?e =ₑ ?f ?a' ?b' ?c' ?d' ?e') =>
+      decide_field a a'; [ .. |
+      decide_field b b'; [ .. |
+      decide_field c c'; [ .. |
+      decide_field d d'; [ .. |
+      decide_field e e'; [ .. |
+      left; reflexivity]]]]]
+  | |- Decision (?f ?a ?b ?c ?d =ₑ ?f ?a' ?b' ?c' ?d') =>
+      decide_field a a'; [ .. |
+      decide_field b b'; [ .. |
+      decide_field c c'; [ .. |
+      decide_field d d'; [ .. |
+      left; reflexivity]]]]
+  | |- Decision (?f ?a ?b ?c =ₑ ?f ?a' ?b' ?c') =>
+      decide_field a a'; [ .. |
+      decide_field b b'; [ .. |
+      decide_field c c'; [ .. |
+      left; reflexivity]]]
+  | |- Decision (?f ?a ?b =ₑ ?f ?a' ?b') =>
+      decide_field a a'; [ .. |
+      decide_field b b'; [ .. |
+      left; reflexivity]]
+  | |- Decision (?f ?a =ₑ ?f ?a') =>
+      decide_field a a'; [ .. |
+      left; reflexivity]
+  | |- Decision (?f =ₑ ?f) => left; reflexivity
+  | |- Decision (_ =ₑ _) => right; discriminate
+  end.
+
+(** * Generic noreturn type
+
+This is intended to mark explicitly effect that are not returning when defining
+custom effects *)
+
+Definition noreturn := False.
+
+#[global] Instance emptyT_noreturn : EmptyT noreturn.
+Proof. inversion 1. Qed.
+
+(** * Non determinism effect *)
+
+(** MChoice is the standard non determinism effect, doing a n-wise choice
+    n can be 0 in which case this correspond to a no-behavior execution *)
+Inductive MChoice : eff := ChooseFin (n : nat) : MChoice (fin n).
+
+#[global] Instance MChoice_EffWd : Eff.Wf MChoice.
+Proof. intros T [[]]; apply _. Qed.
+
+Equations MChoice_EffDec : Eff.Decision MChoice :=
+  MChoice_EffDec _ _ (ChooseFin n) (ChooseFin n') := dec_if (decide (n = n')).
+Solve All Obligations with hauto lq:on.
+#[global] Existing Instance MChoice_EffDec.
+
+Inductive discard_type := discard_value.
+
+(* Not using unit a exception type to be sure that discard is never confused
+   with failing, as mfail is implemented as mthrow unit *)
+#[global] Program Instance MChoice_EffExc : Eff.Exc MChoice :=
+  { exc := discard_type;
+    exc2eff := λ _, existT _ (ChooseFin 0);
+    eff2exc := λ T c,
+      match c return option discard_type with
+      | ChooseFin 0 => Some discard_value
+      | _ => None
+      end
+  }.
+Solve All Obligations with sauto.
+
+(** Special case of MCall for MChoice *)
+Notation MChoose := (MCall MChoice).
+Definition mchoose `{MChoose M} (n : nat) : M (fin n) := mcall (ChooseFin n).
+Definition mdiscard `{MCall MChoice M} `{FMap M} {A} : M A :=
+  mcall (ChooseFin 0) |$> (λ x, match (x : fin 0) with end).
+
+(** Helper to non-deterministically choose in a list *)
+Definition mchoosel `{MChoose M} `{FMap M} {A} (l : list A) : M A :=
+  mchoose (length l) |$> ((list_to_vec l) !!!.).
+
+
+(* TODO add state effects *)
