Common/FMon.v
@@ -1,0 +1,576 @@
+
+Require Import CBase.
+Require Import CResult.
+Require Import Common.
+From stdpp Require Import option.
+
+(* Reexporting Effects. Using FMon implies using Effects *)
+Require Export Effects.
+Open Scope effect_scope.
+
+(* Needed for setoid rewrite along fequiv and cequiv that are defined as an
+   Equiv instance *)
+#[export] Typeclasses Transparent Equiv.
+
+
+
+(** * Free monad
+
+This is a custom implementation of a free monad, which is basically a finite
+itree (thus inductive, not coinductive). Therefore, it cannot represent
+non-termination. *)
+
+Section FMon.
+  Context {Eff : eff}.
+
+  (** This implementation is not very computationally efficient in case of
+      repeated binds, but has the advantage of being canonical up to
+      functional extensionality *)
+  Inductive fMon {A : Type} :=
+  | Ret (ret : A)
+  | Next {T : Type} (call : Eff T) (k : T → fMon).
+  Arguments fMon : clear implicits.
+
+  #[global] Instance fMon_ret : MRet fMon := @Ret.
+
+  #[global] Instance fMon_bind : MBind fMon :=
+    λ _ _, fix bind f ma :=
+      match ma with
+      | Ret x => f x
+      | Next oc k => Next oc (λ x, bind f (k x)) end.
+
+  #[global] Instance fMon_join : MJoin fMon :=
+    λ _ mmx, mx ← mmx; mx.
+
+  #[global] Instance fMon_fmap : FMap fMon :=
+    λ _ _, fix map f ma :=
+      match ma with
+      | Ret x => Ret (f x)
+      | Next oc k => Next oc (λ x, map f (k x)) end.
+
+  #[global] Instance fMon_call : MCall Eff fMon := λ _ out, Next out Ret.
+
+  (** * FMon equivalence
+
+     This would be plain equality with functional extensionality,
+     TODO: maybe we should actually require FunExt and remove this *)
+  Inductive fequiv {A} : Equiv (fMon A) :=
+  | FERet a : fequiv (Ret a) (Ret a)
+  | FENext T (call : Eff T) k1 k2 (Hpr : pointwise_relation T fequiv k1 k2):
+    fequiv (Next call k1) (Next call k2).
+
+  #[global] Instance fequiv_sym A : Symmetric (@fequiv A).
+  Proof using. intros x y H. induction H; constructor; naive_solver. Qed.
+
+  #[global] Instance fequiv_refl A : Reflexive (@fequiv A).
+  Proof using. intros x. induction x; constructor; naive_solver. Qed.
+
+  #[global] Instance fequiv_trans A : Transitive (@fequiv A).
+  Proof using.
+    intros x y z H H'.
+    generalize dependent z.
+    induction H;
+      intros z H';
+      dependent destruction H';
+      constructor;
+      sfirstorder.
+  Qed.
+
+  #[global] Instance fequiv_equiv A : Equivalence (@fequiv A).
+  Proof using. constructor; apply _. Qed.
+
+  #[global] Instance Next_fequiv_Proper A T (call : Eff T):
+    Proper (pointwise_relation T fequiv ==> @fequiv A) (Next call).
+  Proof using. hauto l:on. Qed.
+
+  Infix "≡ₑ" := fequiv (at level 70, no associativity).
+  Infix "≡ₑ@{ A }" := (@fequiv A _)
+                       (at level 70, only parsing, no associativity).
+
+  (** * Events and traces *)
+
+  (** A event of an effect type is a combination of an effect call and its
+      result *)
+  Record fEvent := FEvent {ftype : Type; fcall : Eff ftype; fret: ftype}.
+  Arguments FEvent {_} _ _.
+
+  Infix "&→" := FEvent (at level 45, no associativity).
+
+  (** The type of trace over fMon. Those trace are partial and can stop
+      anywhere *)
+  Inductive fTrace {A : Type} :=
+  | FTNext (ev : fEvent) (ntr : fTrace)
+  | FTRet (a : A)
+  | FTStop {T} (call : Eff T).
+  Arguments fTrace : clear implicits.
+
+  Fixpoint ftlist {A : Type} (ft : fTrace A) :=
+    match ft with
+    | FTNext ev ntr => ev :: ftlist ntr
+    | _ => []
+    end.
+  Fixpoint ftres {A : Type} (ft : fTrace A) : result (sigT Eff) A:=
+    match ft with
+    | FTNext ev ntr => ftres ntr
+    | FTRet a => Ok a
+    | FTStop call => Error (existT _ call)
+    end.
+
+  Fixpoint fTrace_list_res {A} (l : list fEvent) (r : result (sigT Eff) A) :=
+    match l with
+    | [] => match r with
+            | Ok a => FTRet a
+            | Error (existT T call) => FTStop call
+            end
+    | ev :: tl => FTNext ev (fTrace_list_res tl r)
+    end.
+
+  Lemma fTrace_ftlist_ftres {A} (ft : fTrace A) :
+    fTrace_list_res (ftlist ft) (ftres ft) = ft.
+  Proof using. induction ft; sfirstorder. Qed.
+  Hint Rewrite @fTrace_ftlist_ftres : fmon.
+
+  Lemma ftlist_fTrace_list_res {A} l e :
+    ftlist (@fTrace_list_res A l e) = l.
+  Proof using. induction l; hauto lq:on. Qed.
+  Hint Rewrite @ftlist_fTrace_list_res : fmon.
+
+  Lemma ftres_fTrace_list_res {A} l e :
+    ftres (@fTrace_list_res A l e) = e.
+  Proof using. induction l; hauto lq:on. Qed.
+  Hint Rewrite @ftres_fTrace_list_res : fmon.
+
+  (** * Full traces *)
+
+  (** Full trace are traces that only stop on a non returning effect *)
+  Definition ftfull {A} (ft : fTrace A) :=
+    ∀ T call, ftres ft = Error (existT T call) → T → False.
+  Lemma ftfull_FTRet {A} (a : A) : ftfull (FTRet a).
+  Proof using. hfcrush. Qed.
+  Hint Resolve ftfull_FTRet : fmon.
+  Lemma ftfull_FTNext {A} ev (ntr : fTrace A) :
+    ftfull ntr → ftfull (FTNext ev ntr).
+  Proof using. hfcrush. Qed.
+  Hint Resolve ftfull_FTNext : fmon.
+  Lemma ftfull_FTStop {A} T (call : Eff T) :
+    (T → False) → ftfull (A := A) (FTStop call).
+  Proof using. intros H T' call' H'. by dependent destruction H'. Qed.
+  Hint Resolve ftfull_FTStop : fmon.
+  Lemma ftfull_FTStop_spec {A} T (call : Eff T) :
+    ftfull (A := A) (FTStop call) ↔ (T → False).
+  Proof using. split. sfirstorder. apply ftfull_FTStop. Qed.
+  Hint Rewrite @ftfull_FTStop_spec : fmon.
+
+  Equations ftfull_dec {A} `{Eff.Wf Eff} (ft : fTrace A) : Decision (ftfull ft) :=
+    ftfull_dec (FTNext _ tr) := dec_if (ftfull_dec tr);
+    ftfull_dec (FTRet _) := left _;
+    ftfull_dec (@FTStop T call) with decideT T := {
+      | inleft _ => right _
+      | inright _ => left _
+      }.
+  Solve All Obligations with hauto l:on db:fmon.
+
+  (** If the effect type provides an exception type to represent its non
+      terminating calls, then we can use that type to represent a trace *)
+  Context {Ex : Eff.Exc Eff}.
+  Notation exc := (Eff.exc Eff).
+
+  (** If an effect type provide an exception, one can throw that exception
+      This is implemented by a Hint Extern later *)
+  Definition fmon_throw_exc : MThrow exc fMon :=
+    λ _ e, mcall_noret (Eff.exc2eff e).T2.
+
+  Definition ftres_full {A} (ft : fTrace A) : option (result exc A) :=
+    match ftres ft with
+    | Ok a => Some (Ok a)
+    | Error (existT T call) => Eff.eff2exc call |$> Error
+    end.
+
+  Lemma ftres_full_ftfull {A} (ft : fTrace A) :
+    ftfull ft ↔ is_Some (ftres_full ft).
+  Proof using.
+    unfold ftfull, ftres_full.
+    destruct (ftres ft) as [|[]].
+    - hauto l:on.
+    - rewrite fmap_is_Some.
+      rewrite Eff.exc_empty.
+      split.
+      + naive_solver.
+      + injection 2. sfirstorder.
+  Qed.
+
+  Definition fTrace_list_res_full {A} (l : list fEvent) (r : result exc A) :=
+    fTrace_list_res l (mapE Eff.exc2eff r).
+
+  Lemma fTrace_ftlist_ftres_full {A} (ft : fTrace A) e:
+    ftres_full ft = Some e →
+    fTrace_list_res_full (ftlist ft) e = ft.
+  Proof using.
+    unfold fTrace_list_res_full.
+    intro H.
+    rewrite <- fTrace_ftlist_ftres.
+    f_equal.
+    unfold ftres_full, mapE in *.
+    repeat case_split;
+      try (f_equal; rewrite Eff.exc_wf);
+      try (rewrite fmap_Some in * );
+      sfirstorder.
+  Qed.
+  Hint Rewrite @fTrace_ftlist_ftres_full : fmon.
+
+  Lemma ftlist_fTrace_list_res_full {A} l e :
+    ftlist (@fTrace_list_res_full A l e) = l.
+  Proof using. unfold fTrace_list_res_full. hauto l:on db:fmon. Qed.
+  Hint Rewrite @ftlist_fTrace_list_res_full : fmon.
+
+  Lemma ftres_fTrace_list_res_full {A} l e :
+    ftres_full (@fTrace_list_res_full A l e) = Some e.
+  Proof using.
+    unfold fTrace_list_res_full, ftres_full.
+    autorewrite with fmon.
+    destruct e; cbn in *.
+    + done.
+    + case_split.
+      rewrite Eff.exc_wf in *.
+      hauto lq:on.
+  Qed.
+  Hint Rewrite @ftres_fTrace_list_res_full : fmon.
+
+  Lemma ftfull_fTrace_list_res_full A l e: ftfull (A:=A) (fTrace_list_res_full l e).
+  Proof using.
+    rewrite ftres_full_ftfull.
+    by rewrite ftres_fTrace_list_res_full.
+  Qed.
+  Hint Resolve ftfull_fTrace_list_res_full : fmon.
+
+  (** * Trace matching *)
+
+  Inductive fmatch {A : Type} : fMon A → fTrace A → Prop :=
+  | FTMNext T (call : Eff T) k ret tr :
+    fmatch (k ret) tr → fmatch (Next call k) (FTNext (call &→ ret) tr)
+  | FTMRet a : fmatch (Ret a) (FTRet a)
+  | FTMStop T (call : Eff T) k : fmatch (Next call k) (FTStop call).
+
+  Lemma fmatch_next A T (call : Eff T) (k : T → fMon A) (ret : T) tr:
+    fmatch (Next call k) (FTNext (call &→ ret) tr)
+      ↔ fmatch (k ret) tr.
+  Proof using.
+    split; intro H.
+    - dependent destruction H. hauto inv:fTrace.
+    - sauto lq:on.
+  Qed.
+
+  #[global] Instance fmatch_Proper A :
+    Proper (@fequiv A ==> eq ==> iff) fmatch.
+  Proof using.
+    intros m1 m2 H ? t ->.
+    generalize dependent t.
+    induction H.
+    - naive_solver.
+    - split;
+        intro Hfm;
+        dependent destruction Hfm;
+        constructor;
+        naive_solver.
+  Qed.
+
+  Lemma ftrace_exists {A} (m : fMon A) : ∃ t, fmatch m t.
+  Proof using. induction m; hauto q:on ctrs:fmatch. Qed.
+
+  Context {Wf : Eff.Wf Eff}.
+
+  Lemma ftrace_ftfull_exists {A} (m : fMon A) : ∃ t, fmatch m t ∧ ftfull t.
+  Proof using Wf.
+    induction m. hauto lq:on ctrs:fmatch hint:db:fmon.
+    destruct (decideT T).
+    - hauto lq:on ctrs:fmatch.
+    - hauto lq:on ctrs:fmatch db:fmon.
+  Qed.
+
+  Lemma fequiv_via_ftrace_ftfull A m1 m2:
+    (∀ trc : fTrace A, ftfull trc → fmatch m1 trc ↔ fmatch m2 trc) →
+    m1 ≡ₑ m2.
+  Proof using Wf.
+    generalize dependent m2.
+    induction m1; intros m2 Ht; destruct m2.
+    - hauto ctrs:fmatch inv:fmatch q:on db:fmon.
+    - hauto ctrs:fmatch inv:fmatch q:on db:fmon.
+    - hauto ctrs:fmatch inv:fmatch q:on db:fmon.
+    - destruct (ftrace_ftfull_exists (Next call k)) as [tr [Htr Hfull]].
+      pose proof Htr as Htr2.
+      apply Ht in Htr2.
+      dependent destruction Htr;
+      dependent destruction Htr2.
+      + clear dependent tr.
+        constructor.
+        intro a.
+        apply H.
+        intro trc.
+        specialize Ht with (FTNext (call &→ a) trc).
+        by setoid_rewrite fmatch_next in Ht.
+      + constructor. intro. hauto l:on db:fmon.
+      + done.
+  Qed.
+
+  (** * Fmon Handling *)
+
+  Definition fHandler (M : Type → Type) := ∀ A, Eff A → M A.
+
+  Definition mcall_fHandler `{MC : MCall Eff M} : fHandler M := @mcall _ _ MC.
+
+  Fixpoint finterp `{MRet M, MBind M} (handler : fHandler M)
+    [A] (mon : fMon A) : M A :=
+    match mon with
+    | Ret a => (mret a : M A)
+    | @Next _ T call k => ret ←@{M} handler T call; finterp handler (k ret)
+    end.
+
+  #[global] Instance fequiv_finterp A `{MRet M, MBind M} (handler : fHandler M):
+    (∀ T, Proper (pointwise_relation T eq ==> eq ==> eq) (@mbind M _ T A)) →
+    Proper (@fequiv A ==> eq) (finterp handler (A := A)).
+  Proof using.
+    intros P m1 m2 He.
+    induction He; sfirstorder.
+  Qed.
+
+  Lemma finterp_mcall A (f : fMon A) : finterp mcall_fHandler f ≡ₑ f.
+  Proof using. induction f; hauto l:on. Qed.
+
+
+
+  (** * Decidability for fmatch *)
+
+  Context {ED : Eff.Decision Eff}.
+
+  Definition event_extract (ev : fEvent) {T} (call : Eff T) : option T :=
+    match decide (ev.(fcall) =ₑ call) with
+    | left e => Some (Eff.conv_ret (Eff.eq_type e) ev.(fret))
+    | right _ => None
+    end.
+
+  Lemma event_extract_Some ev T (call : Eff T) ret :
+    event_extract ev call = Some ret ↔ ev = (call &→ ret).
+  Proof using.
+    unfold event_extract.
+    case_decide.
+    - pose proof H as H'.
+      simplify_eff_eq in H'.
+      setoid_rewrite UIP_refl.
+      split.
+      + hauto q:on inv:fEvent.
+      + intro E.
+        destruct ev.
+        by dependent destruction E.
+    - hauto q:on.
+  Qed.
+
+  Lemma event_extract_None ev T (call : Eff T) :
+    event_extract ev call = None ↔ fcall ev ≠ₑ call.
+  Proof using.
+    rewrite eq_None_not_Some.
+    apply not_iff_compat.
+    unfold is_Some.
+    setoid_rewrite event_extract_Some.
+    clear Wf Ex. (* Otherwise sauto uses them *)
+    sauto.
+  Qed.
+
+  Equations fmatch_dec `{EqDecision A}
+      (f : fMon A) tr : Decision (fmatch f tr) :=
+    fmatch_dec (Next call k) (FTNext ev ft)
+      with inspect (event_extract ev call) := {
+      | Some ret eq: _ =>
+          dec_if (fmatch_dec (k ret) ft)
+      | None eq: _ => right _
+      } ;
+    fmatch_dec (Ret r) (FTRet r') := dec_if (decide (r = r'));
+    fmatch_dec (Next call k) (FTStop call') := dec_if (decide (call =ₑ call'));
+    fmatch_dec _ _ := right _.
+  Solve All Obligations with
+    intros; cbn in *;
+    try (rewrite event_extract_Some in *;
+         subst ev;
+         by rewrite <- fmatch_next in * );
+    try match goal with | |- ¬ _ => intro H; dependent destruction H end;
+    try(rewrite event_extract_None in * );
+    hauto db:fmon.
+  #[global] Existing Instance fmatch_dec.
+
+End FMon.
+Arguments fMon : clear implicits.
+Arguments fEvent : clear implicits.
+Arguments FEvent {_ _} _ _.
+Arguments fTrace : clear implicits.
+Arguments fHandler : clear implicits.
+#[global] Instance fequiv_params : Params (@fequiv) 2 := {}.
+Infix "≡ₑ" := fequiv (at level 70, no associativity).
+Infix "≡ₑ@{ A }" := (@fequiv A _)
+                      (at level 70, only parsing, no associativity).
+Infix "&→" := FEvent (at level 45, no associativity).
+Infix "&→@{ Eff }" := (@FEvent (Eff _) _) (at level 45, no associativity).
+
+Definition fHandler_plus {Effl Effr : eff} `{MRet M, MBind M}
+    (fl : fHandler Effl M) (fr : fHandler Effr M) : fHandler (Effl +ₑ Effr) M :=
+  λ T e, match e with
+         | inl l => fl T l
+         | inr r => fr T r
+         end.
+Infix "+ₕ" := fHandler_plus (at level 50, left associativity) : effect_scope.
+
+#[export] Hint Extern 5 (MThrow _ ?M) =>
+  let Eff := mk_evar eff in unify M (fMon Eff);
+  class_apply (@fmon_throw_exc Eff _) : typeclass_instances.
+
+(** * Choice monad: Non deterministic free monad *)
+Section CMon.
+  Context {Eff : eff}.
+
+  (** A choice monad is just a free monad with additional choice effects. The
+      only difference is the theory around it (equivalence, trace matching, etc.) *)
+  Definition cMon := fMon (Eff +ₑ MChoice).
+  Notation Nextl e := (Next (inl e)).
+  Notation Nextr e := (Next (inr e)).
+
+  Definition cinterp `{MRet M, MBind M, MChoose M} (f : fHandler Eff M) [A]
+      (c : cMon A) : M A :=
+    finterp (f +ₕ mcall_fHandler) c.
+
+  Definition cmon_throw_exc `{Eff.Exc Eff} : MThrow (Eff.exc Eff) cMon :=
+    λ _ e, @mthrow (Eff.exc Eff + discard_type) _ _ _ (inl e).
+
+  (** * CMon matching with a trace *)
+  Inductive cmatch {A : Type} : cMon A → fTrace Eff A → Prop :=
+  | CTMNext T (call : Eff T) k ret tr :
+    cmatch (k ret) tr → cmatch (Nextl call k) (FTNext (call &→ ret) tr)
+  | CTMChoose n i k tr : cmatch (k i) tr →
+    cmatch (Nextr (ChooseFin n) k) tr
+  | CTMRet a : cmatch (Ret a) (FTRet a)
+  | CTMStop T (call : Eff T) k : cmatch (Nextl call k) (FTStop call).
+
+  #[local] Instance cmatch_fequiv_Proper A :
+    Proper (fequiv ==> eq ==> iff) (@cmatch A).
+  Proof using.
+    intros m1 m2 H ? t ->.
+    generalize dependent t.
+    induction H.
+    - naive_solver.
+    - destruct call as [call | choice];
+        split;
+        intro Hfm;
+        dependent induction Hfm;
+        try (intro H'; dependent destruction H');
+        econstructor;
+        naive_solver.
+  Qed.
+
+  Lemma cmatch_Nextl A T (call : Eff T) (k : T → cMon A) (ret : T) tr:
+    cmatch (Nextl call k) (FTNext (call &→ ret) tr)
+      ↔ cmatch (k ret) tr.
+  Proof using.
+    split; intro H.
+    - dependent destruction H. hauto inv:fTrace.
+    - sauto lq:on.
+  Qed.
+
+  (** Definition of strong equivalence. I haven't found a way to define it in a
+      more useable manner. In particular one can't do an induction on it *)
+  Definition cequiv {A} : Equiv (cMon A) :=
+    λ c1 c2, ∀ tr, cmatch c1 tr ↔ cmatch c2 tr.
+
+  #[local] Instance local_cequiv_params : Params (@cequiv) 1 := {}.
+
+  #[global] Instance cequiv_sym A : Symmetric (@cequiv A).
+  Proof using. unfold Symmetric, cequiv in *. naive_solver. Qed.
+  #[global] Instance cequiv_refl A : Reflexive (@cequiv A).
+  Proof using. unfold Reflexive, cequiv in *. naive_solver. Qed.
+  #[global] Instance cequiv_trans A : Transitive (@cequiv A).
+  Proof using. unfold Transitive, cequiv in *. naive_solver. Qed.
+  #[global] Instance cequiv_equiv A : Equivalence (@cequiv A).
+  Proof using. constructor; apply _. Qed.
+
+  #[global] Instance cequiv_fequiv_Proper A :
+    Proper (fequiv ==> fequiv ==> iff) (@cequiv A).
+  Proof using.
+    unfold cequiv.
+    intros m1 m2 H m'1 m'2 H'.
+    setoid_rewrite H.
+    setoid_rewrite H'.
+    reflexivity.
+  Qed.
+
+  #[global] Instance fequiv_cequiv A : subrelation fequiv (@cequiv A).
+  Proof using. by intros x y ->. Qed.
+
+  #[global] Instance cmatch_cequiv_Proper A :
+    Proper (cequiv ==> eq ==> iff) (@cmatch A).
+  Proof using.
+    intros m1 m2 H ? t ->.
+    by unfold cequiv in H.
+  Qed.
+
+  (** * Some cequiv useability lemma *)
+  Lemma cequiv_Ret A (a : A) : cequiv (Ret a) (Ret a).
+  Proof using. reflexivity. Qed.
+
+  Lemma cequiv_Next A T call k k':
+    pointwise_relation T cequiv k k' → @cequiv A (Next call k) (Next call k').
+  Proof using.
+    intros H trc.
+    destruct call;
+      split;
+      intro Hc;
+      dependent destruction Hc;
+      econstructor;
+      by rewrite H in *.
+  Qed.
+
+  #[global] Instance Next_cequiv_Proper A T call:
+    Proper (pointwise_relation T cequiv ==> @cequiv A) (Next call).
+  Proof using. intros k k'. apply cequiv_Next. Qed.
+
+  (* TODO: Make a good inversion tactic for cequiv *)
+
+  (** * Decidability for cmatch *)
+  Context {ED : Eff.Decision Eff}.
+
+  (** Decide a cmatch: a bit dumb, it will try every possible non-deterministic
+      choice until one match succeeded or all failed. However in practice, if
+      concrete value of cMon avoid doing choice before doing very long
+      identical sequenced of calls in all choice, this shouldn't be that bad. *)
+  Equations cmatch_dec `{EqDecision A} (f : cMon A) tr
+    : Decision (cmatch f tr) :=
+    cmatch_dec (Nextl call k) (FTNext ev ft)
+      with inspect (event_extract ev call) := {
+      | Some ret eq: _ =>
+          dec_if (cmatch_dec (k ret) ft)
+      | None eq: _ => right _
+      } ;
+    cmatch_dec (Ret r) (FTRet r') := dec_if (decide (r = r'));
+    cmatch_dec (Nextl call k) (FTStop call') :=
+      dec_if (decide (call =ₑ call'));
+    cmatch_dec (Nextr (ChooseFin n) k) tr :=
+      dec_if (@decide (∃x : fin n, cmatch (k x) tr) _);
+    cmatch_dec _ _ := right _.
+  Solve Obligations with
+    try (intros; cbn in *;
+         lazymatch goal with | |- Decision _ => fail | |- _ => idtac end;
+         try (rewrite event_extract_Some in *;
+              subst ev;
+              by rewrite <- cmatch_Nextl in * );
+         try match goal with | |- ¬ _ => intro H; dependent destruction H end;
+         try(rewrite event_extract_None in * );
+         hauto ctrs:cmatch).
+  Next Obligation. cbn. intros. apply _. Defined.
+  #[global] Existing Instance cmatch_dec.
+
+End CMon.
+Arguments cMon : clear implicits.
+
+Notation Nextl e := (Next (inl e)).
+Notation Nextr e := (Next (inr e)).
+
+#[global] Instance cequiv_params : Params (@cequiv) 2 := {}.
+
+#[export] Hint Extern 5 (MThrow _ ?M) =>
+  let Eff := mk_evar eff in unify M (cMon Eff);
+  class_apply (@cmon_throw_exc Eff _) : typeclass_instances.
